internal/examples/semantics/nil.go
@@ -14,3 +14,14 @@ func testCompareNilToNil() bool {
 	s := new(*uint64)
 	return *s == nil
 }
+
+func testComparePointerWrappedToNil() bool {
+	var s []byte
+	s = make([]byte, 1)
+	return s != nil
+}
+
+func testComparePointerWrappedDefaultToNil() bool {
+	var s []byte
+	return s == nil
+}
